\begin{multicols}{2}

\subsubsection{Thermodynamics}
\subsubsection{Continuous one-dimensional flow}

\textbf{Thermal equation of state:}
\begin{equation}
\frac{p}{\rho} = RT \quad \text{[term perf]}
\end{equation}

\textbf{Dynamic equation:}
\begin{equation}
\frac{1}{\rho} dp + V dV = 0
\end{equation}

\textbf{Speed of Sound:}
\begin{equation}
a = \sqrt{\left(\frac{\partial p}{\partial \rho}\right)_s} = \sqrt{\gamma \left(\frac{\partial p}{\partial \rho}\right)_T}
\end{equation}

\begin{equation}
a = \sqrt{\gamma \frac{p}{\rho}} = \sqrt{\gamma RT} \quad
\text{[term perf]} \tag{36}
\end{equation}

\textbf{Mach Number:}
\begin{equation}
M = \frac{V}{a}
\end{equation}

\textbf{Dynamic Pressure:}
\begin{equation}
q = \frac{1}{2} \rho V^2
\end{equation}

\begin{equation}
q = \frac{\gamma}{2} p M^2
\end{equation}

From the dynamic equation and the speed of sound relation:
\begin{equation}
\frac{p}{\rho^\gamma} = \text{constant} = \frac{p_t}{\rho_t^\gamma}
\quad \text{[isen, perf]} \tag{34}
\end{equation}

\textbf{From which:}
\begin{equation}
\frac{p}{p_t} = \left(\frac{\rho}{\rho_t}\right)^\gamma = \left(\frac{T}{T_t}\right)^{\frac{\gamma}{\gamma - 1}} = \left(\frac{a}{a_t}\right)^{\frac{2\gamma}{\gamma - 1}}\\
\\ \quad \text{[isen, perf]} \tag{35}
\end{equation}

Combining the above equations gives Bernoulli's equation for compressible flow:
\begin{equation}
\frac{\gamma}{\gamma - 1} \left(\frac{p_t}{\rho_t}\right)^{\frac{\gamma - 1}{\gamma}} \left(\frac{p}{p_t}\right)^{\frac{1}{\gamma}} + \frac{V^2}{2} = \frac{\gamma}{\gamma - 1} \frac{p_t}{\rho_t}
\\ \quad \text{[isen, perf]} \tag{36}
\end{equation}

\textbf{Usefull Ratios}

\begin{gather}
\frac{T}{T_t} = \left(1 + \frac{\gamma - 1}{2} M^2 \right)^{-1}
\quad \text{[adiab, perf]} \tag{43} \\
\frac{p}{p_t} = \left(1 + \frac{\gamma - 1}{2} M^2 \right)^{-\frac{\gamma}{\gamma - 1}}
\quad \text{[isen, perf]} \tag{44} \\
\frac{\rho}{\rho_t} = \left(1 + \frac{\gamma - 1}{2} M^2 \right)^{-\frac{1}{\gamma - 1}}
\quad \text{[isen, perf]} \tag{45} \\
\frac{a}{a_t} = \left(1 + \frac{\gamma - 1}{2} M^2 \right)^{-\frac{1}{2}}
\quad \text{[adiab, perf]} \tag{46}
\end{gather}

\end{multicols}
